heap/pointers added + some organization. All proofs done so far

AssertionSemantics.v.d
@@ -1,2 +1,2 @@
-AssertionSemantics.vo AssertionSemantics.glob AssertionSemantics.v.beautified: AssertionSemantics.v ../CompCert-3.0.1/lib/Coqlib.vo ../CompCert-3.0.1/lib/Integers.vo ../CompCert-3.0.1/lib/Maps.vo ./Environment.vo ./Heap.vo ./Basics.vo ./Expressions.vo
-AssertionSemantics.vio: AssertionSemantics.v ../CompCert-3.0.1/lib/Coqlib.vio ../CompCert-3.0.1/lib/Integers.vio ../CompCert-3.0.1/lib/Maps.vio ./Environment.vio ./Heap.vio ./Basics.vio ./Expressions.vio
+AssertionSemantics.vo AssertionSemantics.glob AssertionSemantics.v.beautified: AssertionSemantics.v ../CompCert-3.0.1/lib/Coqlib.vo ../CompCert-3.0.1/lib/Integers.vo ../CompCert-3.0.1/lib/Maps.vo ./Tactics.vo ./Freshvars.vo ./Environment.vo ./Heap.vo ./Basics.vo ./Expressions.vo
+AssertionSemantics.vio: AssertionSemantics.v ../CompCert-3.0.1/lib/Coqlib.vio ../CompCert-3.0.1/lib/Integers.vio ../CompCert-3.0.1/lib/Maps.vio ./Tactics.vio ./Freshvars.vio ./Environment.vio ./Heap.vio ./Basics.vio ./Expressions.vio
