Environment.v.d
@@ -1,2 +1,2 @@
-Environment.vo Environment.glob Environment.v.beautified: Environment.v ../CompCert-3.0.1/lib/Coqlib.vo ../CompCert-3.0.1/lib/Integers.vo ./Basics.vo
-Environment.vio: Environment.v ../CompCert-3.0.1/lib/Coqlib.vio ../CompCert-3.0.1/lib/Integers.vio ./Basics.vio
+Environment.vo Environment.glob Environment.v.beautified: Environment.v ../CompCert-3.0.1/lib/Coqlib.vo ../CompCert-3.0.1/lib/Integers.vo ./Tactics.vo ./Basics.vo
+Environment.vio: Environment.v ../CompCert-3.0.1/lib/Coqlib.vio ../CompCert-3.0.1/lib/Integers.vio ./Tactics.vio ./Basics.vio
