Freshvars.v.d
@@ -1,0 +1,2 @@
+Freshvars.vo Freshvars.glob Freshvars.v.beautified: Freshvars.v ../CompCert-3.0.1/lib/Coqlib.vo ./Tactics.vo
+Freshvars.vio: Freshvars.v ../CompCert-3.0.1/lib/Coqlib.vio ./Tactics.vio
