AssertionSemantics.v
@@ -9,7 +9,8 @@ Require Import compcert.lib.Coqlib.
 Require Import compcert.lib.Integers.
 Require Import compcert.lib.Maps.
 
-
+Require Import VCC.Tactics.
+Require Import VCC.Freshvars.
 Require Import VCC.Environment.
 Require Import VCC.Heap.
 Require Import VCC.Basics.
@@ -34,16 +35,56 @@ Fixpoint val_type (h:heap)(v:val)(ty:type):Prop:=
     | Tvoid, _ => True 
     | _, None => False
     end 
-  | Vint _, Tint
+  | Vint _, Tint => True
   | _, _ => False
   end.
 
+(*FIXME: seems like this should be moved to Expressions.v*)
 Fixpoint expr_type (ex:expr)(e:env)(h:heap)(ty:type): Prop:=
   match ex with
   | Econst_int _ => ty = Tint
   | Etempvar x => exists v, find e x = Some v /\ val_type h v ty
   | Ederef ex' =>  expr_type ex' e h (Tpointer ty)
   end.
+Lemma eval_expr_type:
+  forall (ex : expr) (e : renv) (h : heap) ty v,
+    eval_expr ex e h v ->
+    val_type h v ty ->
+    expr_type ex e h ty.
+Proof.
+  induction ex; simpl; intros.
+  - destruct_eval_expr.
+    unfold val_type in H0.
+    destruct ty; inversion H0; auto.
+  - destruct_eval_expr.
+    eexists; split; eauto.
+  - destruct_eval_expr.
+    eapply IHex; eauto.
+    invert H2.  
+    simpl; rewrite H.
+    destruct ty; auto.
+Qed.
+Lemma expr_type_eval_pointers:
+  forall ex e h v ty,
+    eval_expr (Ederef ex) e h v ->
+    expr_type ex e h (Tpointer ty) ->
+    val_type h v ty.
+Proof.
+  induction ex;intros; try solve [invert H0].
+  - destruct_eval_expr.
+    destruct_eval_expr.
+    destruct H3 as (?&?&?).
+    rewrite H0 in H; invert H.
+    simpl in H1.
+    invert H2.
+    destruct ty; rewrite H in H3; auto.
+  - simpl in *.
+    destruct_eval_expr.
+    eapply IHex in H1; eauto.
+    simpl in H1.
+    invert H2.
+    destruct ty; rewrite H in H1; auto.
+Qed.
 
 Global Instance Proper_expr_type_expr: Proper (Logic.eq ==> env_equiv ==> Logic.eq ==>Logic.eq ==> Logic.iff) expr_type.
 Proof.
@@ -159,7 +200,7 @@ Fixpoint eval_assert (P:assertion)(re:renv)(rh:heap)(ghe:genv): Prop:=
     ~ rh adr = None
   | (UPDATE p v h2)%assert =>
     exists p_ v_ h2_,
-    find ghe p = Some (GV (GVptr p_)) /\
+    find ghe p = Some (RV (Vptr p_)) /\
     find ghe v = Some (RV v_) /\
     find ghe h2 = Some (GV (GVheap h2_)) /\
     h2_ = update_heap rh p_ (Some v_)
@@ -246,14 +287,6 @@ Proof.
 Qed.
 
 (** *Tactics *)
-Ltac destruct_and:=
-  repeat match goal with
-         | [ H: _ /\ _  |- _ ] => destruct H
-         end.
-Ltac reduce_and:=
-  repeat match goal with
-         | [ |- _ /\ _  ] => split
-         end.
 Ltac destruct_list_entailment:=
   repeat match goal with
          | [ H: list_entailment (_ :: _)  |- _ ] =>
@@ -299,40 +332,59 @@ Ltac entailer:=
 
 
 Section FreeFreshVars.
-(** 
+  (** 
    Free variables and fresh variables for assertions:
    Free variables are all ID's in the assertions that are not bound
    to a quantifier.
    Fresh variables are variables not in the fresh set. 
- *)
+   *)
   (** THIS IS ONLY ABOUT TEMPORAL LOCAL VARIABLES*)
+  Definition fresh_var (set_vars:PSet.t): positive:=
+    match (max_elt set_vars) with
+    | Some x => x~1
+    | None => 1
+    end.
 
-Fixpoint free_vars (A: assertion): PSet.t:= (*returns a set od positives*)
-  match A with
-  | Atrue | Afalse=> empty
-  | Aand A1 A2 => union (free_vars A1) (free_vars A2)
-  | Aor A1 A2 => union (free_vars A1) (free_vars A2)
-  | Anot A' => free_vars A'
-  | Aexists id A' => (free_vars A')
-  | Agexists x A' => PSet.remove x (free_vars A')
-  | Adefined id => empty
-  | Agdefined id => singleton id
-  | Aalloc p => singleton p
-  | (UPDATE p v h2)%assert => union (singleton p) (union (singleton v) (singleton h2))
-  | Aexists_heap A' => free_vars A'
-  | Aequal_heap xh => singleton xh
-  | Aexpr_type e _ => empty
-  | Agexpr_type ex _ => free_vars_expr ex
-  | Aref_eq ex1 ex2 => union (free_vars_expr ex1) (free_vars_expr ex2)
-  | Aeq ex1 ex2 => union (free_vars_expr ex1) (free_vars_expr ex2)
-  end.
+  (* Simplify hypothesis of the form context[In x s] *)
+  Ltac simpl_set HH:=
+    repeat first
+           [rewrite union_spec in HH |
+            rewrite singleton_spec in HH];
+    normal_form_not_or.
 
-Definition env_equiv_assert (P:assertion): relation genv:=
-  fun e1 e2 =>
-    forall x, PSet.In x (free_vars P) ->
-         (find e1 x) = (find e2 x).
+  (* Simplify goal of the form [~ In x s] *)
+  Ltac reduce_in_set:=
+    repeat first[ rewrite union_spec;
+                  try (eapply Classical_Prop.and_not_or; split)|
+                  rewrite singleton_spec ].
+  
+  Fixpoint free_vars (A: assertion): PSet.t:= (*returns a set od positives*)
+    match A with
+    | Atrue | Afalse=> empty
+    | Aand A1 A2 => union (free_vars A1) (free_vars A2)
+    | Aor A1 A2 => union (free_vars A1) (free_vars A2)
+    | Anot A' => free_vars A'
+    | Aexists id A' => (free_vars A')
+    | Agexists x A' => PSet.remove x (free_vars A')
+    | Adefined id => empty
+    | Agdefined id => singleton id
+    | Aalloc p => singleton p
+    | (UPDATE p v h2)%assert => union (singleton p) (union (singleton v) (singleton h2))
+    | Aexists_heap A' => free_vars A'
+    | Aequal_heap xh => singleton xh
+    | Aexpr_type e _ => empty
+    | Agexpr_type ex _ => free_vars_expr ex
+    | Aref_eq ex1 ex2 => union (free_vars_expr ex1) (free_vars_expr ex2)
+    | Aeq ex1 ex2 => union (free_vars_expr ex1) (free_vars_expr ex2)
+    end.
 
-Global Instance Equivalenc_env_equiv_assert: forall ass, Equivalence (env_equiv_assert ass).
+  Definition env_equiv_assert (P:assertion): relation genv:=
+    fun e1 e2 =>
+      forall x, PSet.In x (free_vars P) ->
+           (find e1 x) = (find e2 x).
+
+  Global Instance Equivalenc_env_equiv_assert:
+    forall ass, Equivalence (env_equiv_assert ass).
   Proof.
     constructor.
     - constructor.
@@ -344,149 +396,251 @@ Global Instance Equivalenc_env_equiv_assert: forall ass, Equivalence (env_equiv_
     forall e1 e2 ex,
       env_equiv e1 e2 ->
       env_equiv_assert ex e1 e2.
-    Proof. intros ? ? ? H ? ?; apply H. Qed.
+  Proof. intros ? ? ? H ? ?; apply H. Qed.
 
-    Lemma free_vars_env_equiv_assert:
-      forall P k e,
-        ~ PSet.In k (free_vars P) ->
-        forall ov,
-          env_equiv_assert P (update_env e k ov) e.
-    Proof.
-      induction P; intros ? ? ? ? ? ?;
-                          destruct (peq k x); subst;
-        try tauto;
-        rewrite gso; auto.
-    Qed.
-    
-    Global Instance Proper_eval_assert_assert:
-      forall ass, Proper (env_equiv ==> Logic.eq ==> env_equiv_assert ass ==> Logic.iff)
-                    (eval_assert ass).
-    Proof.
-      intros ? ? ? ? ? ? ? ? ? ?; subst.
-      revert y0 x y H x1 y1 H1.
-      induction ass; intros;
-        try solve[split;auto];
-        simpl; intros;
-          try solve[
-                repeat match goal with
-                       | [ H: context[ _ <-> _ ] |- _ ] =>
-                         rewrite H; clear H
-                       end; eauto;
-                try reflexivity;
-                match goal with
-                | [ H: env_equiv_assert _ _ _  |- env_equiv_assert _ _ _ ] =>
-                  intros ? ?; apply H;
-                  simpl; try rewrite PSet.union_spec; auto
-                end];
-          try (apply forall_exists_iff); intros. (*8 goals left*)
-      - eapply IHass; auto; rewrite H; reflexivity.
-      - eapply IHass; auto.
-        intros x' ?; destruct (peq i x'); subst;
-          try do 2 rewrite gss by auto;
-          try do 2 rewrite gso by auto; auto.
-        eapply H1. simpl.
-        apply PSet.remove_spec; split; auto.
-      - try rewrite H; try rewrite H1; reflexivity.
-      - try rewrite H; try rewrite H1. reflexivity.
-        apply singleton_spec; reflexivity.
-      - try rewrite H; try rewrite H1. reflexivity.
-        apply singleton_spec; reflexivity.
-      - repeat (apply forall_exists_iff; intros).
-        repeat rewrite H1; try reflexivity;
+  Lemma free_vars_env_equiv_assert:
+    forall P k e,
+      ~ PSet.In k (free_vars P) ->
+      forall ov,
+        env_equiv_assert P (update_env e k ov) e.
+  Proof.
+    induction P; intros ? ? ? ? ? ?;
+                        destruct (peq k x); subst;
+      try tauto;
+      rewrite gso; auto.
+  Qed.
+
+  Global Instance Proper_eval_assert_assert:
+    forall ass, Proper (env_equiv ==> Logic.eq ==> env_equiv_assert ass ==> Logic.iff)
+                  (eval_assert ass).
+  Proof.
+    intros ? ? ? ? ? ? ? ? ? ?; subst.
+    revert y0 x y H x1 y1 H1.
+    induction ass; intros;
+      try solve[split;auto];
+      simpl; intros;
+        try solve[
+              repeat match goal with
+                     | [ H: context[ _ <-> _ ] |- _ ] =>
+                       rewrite H; clear H
+                     end; eauto;
+              try reflexivity;
+              match goal with
+              | [ H: env_equiv_assert _ _ _  |- env_equiv_assert _ _ _ ] =>
+                intros ? ?; apply H;
+                simpl; try rewrite PSet.union_spec; auto
+              end];
+        try (apply forall_exists_iff); intros. (*8 goals left*)
+    - eapply IHass; auto; rewrite H; reflexivity.
+    - eapply IHass; auto.
+      intros x' ?; destruct (peq i x'); subst;
+        try do 2 rewrite gss by auto;
+        try do 2 rewrite gso by auto; auto.
+      eapply H1. simpl.
+      apply PSet.remove_spec; split; auto.
+    - try rewrite H; try rewrite H1; reflexivity.
+    - try rewrite H; try rewrite H1. reflexivity.
+      apply singleton_spec; reflexivity.
+    - try rewrite H; try rewrite H1. reflexivity.
+      apply singleton_spec; reflexivity.
+    - repeat (apply forall_exists_iff; intros).
+      repeat rewrite H1; try reflexivity;
         clear; simpl;
           repeat (try rewrite union_spec; try rewrite singleton_spec); tauto.
-      - apply IHass; auto.
-      - rewrite H1; simpl; try apply singleton_spec; reflexivity.
-      - rewrite H; reflexivity.
-      - rewrite H; rewrite H1; reflexivity.
+    - apply IHass; auto.
+    - rewrite H1; simpl; try apply singleton_spec; reflexivity.
+    - rewrite H; reflexivity.
+    - rewrite H; rewrite H1; reflexivity.
 
-      - assert (HH: env_equiv_gexpr g x1 y1).
-        { intros ? ?. eapply H1. simpl. apply PSet.union_spec; auto. }
-        assert (HH': env_equiv_gexpr g0 x1 y1).
-        { intros ? ?. eapply H1. simpl; apply PSet.union_spec; auto. }
-        intros; f_equiv; rewrite H;
+    - assert (HH: env_equiv_gexpr g x1 y1).
+      { intros ? ?. eapply H1. simpl. apply PSet.union_spec; auto. }
+      assert (HH': env_equiv_gexpr g0 x1 y1).
+      { intros ? ?. eapply H1. simpl; apply PSet.union_spec; auto. }
+      intros; f_equiv; rewrite H;
         try rewrite HH; try rewrite HH'; reflexivity.
 
-      - assert (HH: env_equiv_gexpr g x1 y1).
-        { intros ? ?. eapply H1. simpl. apply PSet.union_spec; auto. }
-        assert (HH': env_equiv_gexpr g0 x1 y1).
-        { intros ? ?. eapply H1. simpl; apply PSet.union_spec; auto. }
-        
-        intros; f_equiv; rewrite H;
+    - assert (HH: env_equiv_gexpr g x1 y1).
+      { intros ? ?. eapply H1. simpl. apply PSet.union_spec; auto. }
+      assert (HH': env_equiv_gexpr g0 x1 y1).
+      { intros ? ?. eapply H1. simpl; apply PSet.union_spec; auto. }
+      
+      intros; f_equiv; rewrite H;
         try rewrite HH; try rewrite HH'; reflexivity.
 
-Qed.
+  Qed.
 
-Definition fresh_var (set_vars:PSet.t): positive:=
-  match (max_elt set_vars) with
-  | Some x => x~1
-  | None => 1
-  end.
+  Lemma fresh_var_spec:
+    forall set_vars,
+      ~ PSet.In (fresh_var set_vars) set_vars.
+  Proof.
+    intros.
+    cbv delta[fresh_var] beta iota zeta; intros AA.
+    destruct (max_elt set_vars) eqn:BB.
+    - eapply PSet.max_elt_spec2 in BB; eauto.
+      apply BB; eauto.
+      simpl.
+      unfold elt in *.
+      clear.
+      induction e; simpl ; auto.
+    - apply PSet.max_elt_spec3 in BB.
+      eapply BB; eauto.
+  Qed.
 
+  (*Usefull case for assignment case*)
+  Lemma fresh_vars_spec_util:
+    forall phi x ex,
+      let temp:=
+          fresh_var (union (free_vars phi)
+                           (union (free_vars_expr ex) (singleton x)))  in
+      ~ PSet.In temp (free_vars phi) /\
+      ~ PSet.In temp (free_vars_expr ex) /\
+      temp <> x.
+  Proof.
+    intros.
+    pose proof (fresh_var_spec (union (free_vars phi) (union (free_vars_expr ex) (singleton x)))). 
+    do 2 rewrite PSet.union_spec in H.
+    apply Classical_Prop.not_or_and in H; destruct H as [A H].
+    apply Classical_Prop.not_or_and in H; destruct H as [B C].
+    split; auto.
+    split; auto.
+    intros HH; apply C.
+    rewrite PSet.singleton_spec; auto.
+  Qed.
 
-Lemma fresh_var_spec:
-  forall set_vars,
-    ~ PSet.In (fresh_var set_vars) set_vars.
-Proof.
-  intros.
-  cbv delta[fresh_var] beta iota zeta; intros AA.
-  destruct (max_elt set_vars) eqn:BB.
-  - eapply PSet.max_elt_spec2 in BB; eauto.
-    apply BB; eauto.
-    simpl.
-    unfold elt in *.
-    clear.
-    induction e; simpl ; auto.
-  - apply PSet.max_elt_spec3 in BB.
-    eapply BB; eauto.
-Qed.
+  Lemma expr_type_update:
+    forall k gex,
+      ~ PSet.In k (free_vars_expr gex) -> 
+      forall e h ghe ty v_ty, gexpr_type gex e h (update_env ghe k v_ty) ty <->
+                         gexpr_type gex e h ghe ty.
+  Proof.
+    intros; eapply free_vars_env_equiv in H; rewrite H; reflexivity.
+  Qed.
 
-(*Usefull case for assignment case*)
-Lemma fresh_vars_spec_util:
-  forall phi x ex,
-    let temp:= fresh_var (union (free_vars phi) (union (free_vars_expr ex) (singleton x)))  in
-    ~ PSet.In temp (free_vars phi) /\
-    ~ PSet.In temp (free_vars_expr ex) /\
-    temp <> x.
-Proof.
-  intros.
-  pose proof (fresh_var_spec (union (free_vars phi) (union (free_vars_expr ex) (singleton x)))). 
-  do 2 rewrite PSet.union_spec in H.
-  apply Classical_Prop.not_or_and in H; destruct H as [A H].
-  apply Classical_Prop.not_or_and in H; destruct H as [B C].
-  split; auto.
-  split; auto.
-  intros HH; apply C.
-  rewrite PSet.singleton_spec; auto.
-Qed.
+  Lemma eval_expr_update:
+    forall k gex,
+      ~ PSet.In k (free_vars_expr gex) -> 
+      forall e h ghe v v', 
+        eval_gexpr gex e h (update_env ghe k v') v <->
+        eval_gexpr gex e h ghe v.
+  Proof.
+    intros; eapply free_vars_env_equiv in H; rewrite H; reflexivity.
+  Qed.
 
-Lemma expr_type_update:
-  forall k gex,
-    ~ PSet.In k (free_vars_expr gex) -> 
-    forall e h ghe ty v_ty, gexpr_type gex e h (update_env ghe k v_ty) ty <->
-                 gexpr_type gex e h ghe ty.
-Proof.
-  intros; eapply free_vars_env_equiv in H; rewrite H; reflexivity.
-Qed.
-
-Lemma eval_expr_update:
-  forall k gex,
-    ~ PSet.In k (free_vars_expr gex) -> 
-    forall e h ghe v v', 
-      eval_gexpr gex e h (update_env ghe k v') v <->
-      eval_gexpr gex e h ghe v.
-Proof.
-  intros; eapply free_vars_env_equiv in H; rewrite H; reflexivity.
-Qed.
-
-Lemma free_vars_update:
-  forall k phi,
-    ~ PSet.In k (free_vars phi) -> 
-    forall e h ghe v, 
-      eval_assert phi e h (update_env ghe k v) <->
-      eval_assert phi e h ghe.
-Proof.
-  intros; eapply free_vars_env_equiv_assert in H; rewrite H; reflexivity.
-Qed.
+  Lemma free_vars_update:
+    forall k phi,
+      ~ PSet.In k (free_vars phi) -> 
+      forall e h ghe v, 
+        eval_assert phi e h (update_env ghe k v) <->
+        eval_assert phi e h ghe.
+  Proof.
+    intros; eapply free_vars_env_equiv_assert in H; rewrite H; reflexivity.
+  Qed.
 
 End FreeFreshVars.
+
+
+(** *Tactics: simplifing and solving fresh/free variables goals/hypothesis*)
+
+(* Solves goals of the form [fresh_var ?st <> _ ] *)
+Ltac solve_fresh_var_neq':=
+  match goal with
+  | [ |- fresh_var ?st <> _ ] =>
+    let HH := fresh "HH" in
+    pose proof (fresh_var_spec st) as HH;
+    simpl_set HH; assumption
+  end.
+Ltac solve_fresh_var_neq:=
+  first [solve_fresh_var_neq' | symmetry; solve_fresh_var_neq'].
+
+(* simplifies goal and hypothesis of the form [find _ _ = Some _] *)
+(* It replaces subst_find*)
+Ltac simpl_find :=
+  repeat match goal with
+         | [ H: find ?e ?x = Some _, H': find ?e ?x = Some _  |- _ ] =>
+           rewrite H in H'; invert H'
+         | [  |- find _ _ = _ ] =>
+           first [ rewrite gss | rewrite gso by solve_fresh_var_neq]
+         | [ H: find _ _ = Some _  |- _ ] =>
+           first [ rewrite gss in H | rewrite gso in H by solve_fresh_var_neq]
+         end.
+
+(* solves goals of the forma [~ In (fresh_var s1) s2] when s2 < s1*)
+Ltac fresh_var_subset:=
+  match goal with
+  | [ |- ~ PSet.In (fresh_var ?st) _ ] =>
+    let HH := fresh "HH" in
+    pose proof (fresh_var_spec st) as HH;
+    simpl_set HH;
+    reduce_in_set; assumption
+  end.
+
+(* solves goals of the form [~ In x s] *)
+Ltac solve_in_set:=
+  solve [ simpl; reduce_in_set;
+          first[ apply empty_spec
+               | solve[rewrite singleton_spec; solve_fresh_var_neq]
+               | solve[apply fresh_var_spec]
+               | fresh_var_subset] ].
+
+
+(* Simplify the ghost environment in expressions   *)
+Ltac simpl_free_vars_env_equiv:=
+  progress (repeat
+              first[ rewrite free_vars_env_equiv by solve_in_set |
+                     rewrite update_comm by solve_fresh_var_neq;
+                     rewrite free_vars_env_equiv by solve_in_set |
+                     rewrite redundant_update ]).
+Ltac simpl_free_vars_env_equiv_hyp H:=
+  progress (repeat
+              first[ rewrite free_vars_env_equiv in H by solve_in_set |
+                     rewrite update_comm in H by solve_fresh_var_neq;
+                     rewrite free_vars_env_equiv in H by solve_in_set |
+                     rewrite redundant_update]).
+
+(*will try to use commutativity once. *)
+Ltac simpl_env_gexpr:=
+  repeat match goal with
+         | [  |- eval_gexpr _ _ _ _ _ ] =>
+           simpl_free_vars_env_equiv
+         | [  |- eval_glvalue _ _ _ _ _ ] => 
+           simpl_free_vars_env_equiv
+         | [ H: eval_gexpr _ _ _ _ _  |- _ ] => 
+           simpl_free_vars_env_equiv_hyp H
+         | [ H: eval_glvalue _ _ _ _ _  |- _ ] => 
+           simpl_free_vars_env_equiv_hyp H
+         end.
+
+(* Simplify the ghost environment in assertions*)
+Ltac simpl_free_vars_env_equiv_assert:=
+  progress (repeat
+              first[ rewrite free_vars_env_equiv_assert by solve_in_set |
+                     rewrite update_comm by solve_fresh_var_neq;
+                     rewrite free_vars_env_equiv_assert by solve_in_set |
+                     rewrite redundant_update |
+                     rewrite pointless_update by reflexivity ]).
+Ltac simpl_free_vars_env_equiv_assert_hyp H:=
+  progress (repeat
+              first[ rewrite free_vars_env_equiv_assert in H by solve_in_set |
+                     rewrite update_comm in H by solve_fresh_var_neq;
+                     rewrite free_vars_env_equiv_assert in H by solve_in_set|
+                     rewrite redundant_update in H |
+                     rewrite pointless_update in H by reflexivity]).
+
+(** * Some tactics (worth moving some) *)
+Ltac simpl_env_assertion:=
+  repeat match goal with
+         | [  |- eval_assert _ _ _ _ ] =>
+           simpl_free_vars_env_equiv_assert
+         | [ H: eval_assert _ _ _ _ |- _ ] =>
+           simpl_free_vars_env_equiv_assert_hyp H
+         end.
+Ltac solve_assertion_subgoal:=
+  first [ assumption |
+          solve[ simpl_env_gexpr; trivial] |
+          solve [simpl_find; trivial] |
+          solve [simpl_env_assertion; entailer] ].
+Ltac solve_assertion:=
+  first [ solve_assertion_subgoal |
+          (* This second part should be replaced by gexpr_entailer*)
+          try destruct_eval_gexpr;
+          econstructor; solve_assertion_subgoal].
