ExpressionVerifier.v
@@ -1,0 +1,101 @@
+Require Import compcert.lib.Coqlib.
+Require Import compcert.lib.Integers.
+
+Require Import  Program.Equality.
+
+Require Import MSets.MSetPositive.
+Import PositiveSet. Module PSet:= PositiveSet. (*For positive-indexed sets*)
+Require Import Coq.Classes.Morphisms.
+
+Require Import VCC.Tactics.
+Require Import VCC.Basics. Import Basics.
+Require Import VCC.Expressions.
+Require Import VCC.Environment.
+Require Import VCC.Heap.
+Require Import VCC.Semantics.
+Require Import VCC.AssertionSemantics.
+Import Expressions.
+
+
+(*An expressions are defined*)
+Fixpoint assert_expr_defined (ex:expr): assertion:=
+  match ex with
+    Econst_int v => Atrue
+  | Etempvar id => Adefined id
+  | Ederef ex' =>
+    let p:= fresh_var empty in
+    (Agexists p ((GEtempvar p)== ex' /\ Aalloc p))%assert
+  end.
+Fixpoint assert_gexpr_defined (ex:gexpr): assertion:=
+  match ex with
+  | Rexpr ex' => assert_expr_defined ex'
+  | GEconst_ptr p =>
+    let xp:= fresh_var empty in
+    (Agexists xp ((Etempvar xp)== GEconst_ptr p) /\ Aalloc xp)%assert 
+  | GEconst_nat _ => Atrue
+  | GEconst_bool _ => Atrue
+  | GEtempvar id => Agdefined id
+  | GEderef ex' => 
+    let xp:= fresh_var (free_vars_expr ex' ) in
+    (Agexists xp ((GEtempvar xp)== ex' /\ Aalloc xp))%assert
+  end.
+Fixpoint assert_lvalue_defined (ex:expr): assertion:=
+  match ex with
+    Econst_int v => Afalse
+  | Etempvar id => Afalse
+  | Ederef ex' =>
+    let xp:= fresh_var empty in
+    (Agexists xp ((Etempvar xp)== ex'))%assert
+  end.
+
+(* Correctness the previous three functions*)
+Lemma expr_defined_safe:
+  forall (ex : expr) ghe (e : env) (h : heap),
+    [e, h, ghe]|= (assert_expr_defined ex) ->
+    exists v, eval_expr ex e h v.
+Proof.
+  induction ex; try solve[do 2 econstructor];
+    intros ? ? ? H.
+  - simpl in H;
+      destruct (find e id) eqn:HH; [|contradict H; reflexivity].
+    eexists; econstructor; eauto.
+  - destruct H as (v1 &( v2 & ? & ?) & adr & ? & ?).
+    destruct (h adr) eqn:HH; [|contradiction H2; reflexivity].
+    eexists; econstructor;
+      econstructor; try eassumption.
+    fold_eval_expr.
+    simpl_env_gexpr.
+    remember (fresh_var empty) as p.
+    remember (eval_gexpr ex e h ghe v2) as HH0.
+    destruct_eval_gexpr.
+    subst HH0.
+    destruct_eval_expr.
+    simpl_find.
+    invert H0; eauto.
+    eapply eval_gexpr_expr; eauto.
+Qed.
+Lemma gexpr_defined_safe:
+  forall (ex : gexpr) ghe (e : env) (h : heap),
+    [e, h, ghe]|= (assert_gexpr_defined ex) ->
+    exists v, eval_gexpr ex e h ghe v.
+Proof.
+  induction ex; try solve[do 2 econstructor];
+    intros ? ? ? H.
+  - eapply expr_defined_safe in H as (?&?).
+    do 2 econstructor; eauto.
+  - simpl in H.
+    destruct (find ghe id) eqn:HH; [|contradict H; reflexivity].
+    eexists; econstructor; eauto.
+  - destruct H as (v1 &( v2 & ? & ?) & adr & ? & ?).
+    destruct (h adr) eqn:HH; [|contradiction H2; reflexivity].
+    eexists; econstructor;
+      econstructor; try eassumption.
+    fold_eval_gexpr.
+    remember (fresh_var empty) as p.
+    simpl_env_gexpr.
+    remember (eval_gexpr ex e h ghe v2) as HH0.
+    destruct_eval_gexpr.
+    subst HH0.
+    simpl_find.
+    assumption.
+Qed.
