Freevars.v
@@ -1,0 +1,10 @@
+(*For finite sets*)
+Require Import MSets.MSetPositive.
+Import PositiveSet. Module PSet:= PositiveSet. (*For positive-indexed sets*)
+Require Import Coq.Classes.Morphisms.
+
+Definition fresh_var (set_vars:PSet.t): positive:=
+  match (max_elt set_vars) with
+  | Some x => x~1
+  | None => 1
+  end.
