Tactics.v
@@ -1,0 +1,47 @@
+
+Require Import Coq.Logic.Classical_Prop.
+Require Import Coq.Classes.RelationClasses.
+Require Import Coq.Relations.Relation_Definitions.
+
+
+(* neq is reflexive. *)
+Definition neq_rel (A:Type): relation A:=
+  fun (x y:A) => x <> y.
+Global Instance Symmetric_neq: forall A, @Symmetric A (neq_rel A).
+Proof. intros ? ? ? H ?. apply H; auto. Qed.
+
+(* Duplicate hypothesis *)
+Ltac duplicate H:= let HH := fresh "HH" in assert (HH:=H).
+
+(* "Normal form"  hypothesis*)
+Ltac normal_form_not_or:=
+  repeat match goal with
+         | [ H: ~ ( _ \/ _ ) |- _ ] =>
+           apply Classical_Prop.not_or_and in H; destruct H
+         end.
+Ltac destruct_and:=
+  repeat match goal with
+         | [ H: _ /\ _  |- _ ] => destruct H
+         end.
+Ltac reduce_and:=
+  repeat match goal with
+         | [ |- _ /\ _  ] => split
+         end.
+
+(* Stronger form of inversion *)
+(* It inverts and rewrites every *new* equality*)
+(* NOTE!!: This changes the names of hypothesis!!! *)
+(* I considere good practice to not depend on names*)
+Ltac revert_but HH:=
+  repeat match goal with
+         | [ H: _ |- _ ] =>
+           progress
+             match H with
+             | HH => idtac
+             | _ => revert H
+             end
+         end.
+Ltac invert HH:=
+  revert_but HH;
+  inversion HH; subst;
+  intros.
